\chapter{Space Complexity Fingertrees \label{chap:spacecomp}}
The equation in \cref{fig:bla} describes the how the space complexity for the
measures in a fingertree is reached.
\begin{figure}[!h]
\begin{center}
$\sum\limits_{x=0}^{\log (n-1)}(n- 2 \cdot \sum\limits_{y=1}^x2^y) =
n + n \log(n-1) - \sum\limits_{x=0}^{\log (n-1)} 2 \cdot \sum\limits_{y=1}^{x} 2^y=
n + n \log(n-1) - \sum\limits_{x=0}^{\log (n-1)} 2(2^{x+1} - 2) =
n + n \log(n-1) - \sum\limits_{x=0}^{\log (n-1)} (2^{x+2} - 4) =
n + n\log(n-1) + 4\log(n-1) + 4 - \sum\limits_{x=0}^{\log(n-1)} 2^{x+2} =
n + (n+4)\log(n-1) - 2^{\log(n-1)+3} +8 =
n + (n+4)\log(n-1) - 8(n-1) + 8=
(n+4)\log(n-1) - 7n + 16 \Rightarrow \Theta(n\log n)$
\end{center}
\caption{The number of characters being measured in a tree with n characters\label{fig:bla}}
\end{figure}
